formalization/FinalProcess.v
@@ -1,0 +1,1423 @@
+From FD Require Import Syntax.
+From FD Require Import Types.
+From FD Require Import Renaming.
+From FD Require Import StructCong.
+From FD Require Import Reduction.
+From FD Require Import Contexts.
+From FD Require Import Typing.
+From FD Require Import FreeVars.
+
+From Stdlib Require List.
+From Stdlib Require Import PeanoNat.
+From Stdlib Require Import Lia.
+Import List.ListNotations.
+
+(******************************************************************************)
+(* Canonical Cut Forms                                                        *)
+(******************************************************************************)
+Definition no_root_cut (P : process) :=
+  forall Q R, P <> (cut Q R).
+
+Inductive cut_list : process -> Prop :=
+  | cut_list_nil  : forall L R,
+                      no_root_cut L ->
+                      no_root_cut R ->
+                      cut_list (cut L R)
+  | cut_list_cons : forall L P,
+                      no_root_cut L ->
+                      cut_list P ->
+                      cut_list (cut L P).
+
+(******************************************************************************)
+(* Final Processes                                                            *)
+(******************************************************************************)
+Inductive link_list : list nat -> process -> Prop :=
+  | link_cut_ll : forall i1 i2 M1 M2,
+                    link_list [i1; i2] (cut (link (future i1) M1) (link (future i2) M2))
+  | link_cut_lr : forall i1 i2 M1 M2,
+                    link_list [i1; i2] (cut (link (future i1) M1) (link M2 (future i2)))
+  | link_cut_rl : forall i1 i2 M1 M2,
+                    link_list [i1; i2] (cut (link M1 (future i1)) (link (future i2) M2))
+  | link_cut_rr : forall i1 i2 M1 M2,
+                    link_list [i1; i2] (cut (link M1 (future i1)) (link M2 (future i2)))
+  | link_cons_l   : forall i M xs P,
+                      link_list (List.map S xs) P ->
+                      link_list (i :: xs) (cut (link (future i) M) P)
+  | link_cons_r   : forall i M xs P,
+                      link_list (List.map S xs) P ->
+                      link_list (i :: xs) (cut (link M (future i)) P).
+
+(* Inductive link_list : list nat -> process -> Prop :=
+  | link_single_l : forall i M, link_list [i] (link (future i) M)
+  | link_single_r : forall i M, link_list [i] (link M (future i))
+  | link_cons_l   : forall i M xs P,
+                      link_list (List.map S xs) P ->
+                      link_list (i :: xs) (cut (link (future i) M) P)
+  | link_cons_r   : forall i M xs P,
+                      link_list (List.map S xs) P ->
+                      link_list (i :: xs) (cut (link M (future i)) P). *)
+
+Inductive final : process -> Prop :=
+  | final_stop : final stop
+  | final_future_l : forall i M, final (link (future i) M)
+  | final_future_r : forall i M, final (link M (future i))
+  | final_list : forall xs P P',
+                  ~ (List.In 0 xs) ->
+                  (* (forall x, List.In x xs -> x <> 0) -> *)
+                  link_list xs P' ->
+                  P ≡ P' ->
+                  final P.
+
+(******************************************************************************)
+(* Canonical Cut Form                                                         *)
+(******************************************************************************)
+Lemma renaming_preserves_cut_listness :
+  forall P r,
+    cut_list P -> cut_list (rename_process P r).
+Proof.
+  intros.
+  generalize dependent r.
+  induction H; intros; simpl.
+  + apply cut_list_nil.
+    - destruct L; simpl; congruence.
+    - destruct R; simpl; congruence.
+  + apply cut_list_cons.
+    - destruct L; simpl; congruence.
+    - apply IHcut_list.
+Qed.
+
+Lemma upshifting_preserves_cut_listness :
+  forall P k n,
+    cut_list P -> cut_list (lift_process P k n).
+Proof.
+  intros.
+  generalize dependent k.
+  generalize dependent n.
+  induction H; intros; simpl.
+  + apply cut_list_nil; try destruct L; try destruct R; simpl; congruence.
+  + apply cut_list_cons.
+    - destruct L; simpl; congruence.
+    - apply IHcut_list.
+Qed.
+
+Lemma downshift_preserves_cut_listness :
+  forall P n,
+    cut_list P -> cut_list (down1_process P n).
+Proof.
+  intros.
+  generalize dependent n.
+  induction H; intros; simpl.
+  + apply cut_list_nil; try destruct L; try destruct R; simpl; congruence.
+  + apply cut_list_cons.
+    - destruct L; simpl; congruence.
+    - apply IHcut_list.
+Qed.
+
+Lemma cut_lists_flatten_in_cut' :
+  forall n Γ P Q,
+  forall k,
+    k <= n ->
+    depth P = k ->
+    Γ ⊢ (cut P Q) :# ->
+    cut_list P ->
+    cut_list Q ->
+    exists R, (cut P Q) ≡ R /\ cut_list R.
+Proof.
+  induction n; intros.
+  + destruct P; exfalso.
+    - inversion H2.
+    - simpl in H0. rewrite <- H0 in H. inversion H.
+    - simpl in H0. rewrite <- H0 in H. inversion H.
+    - inversion H2.
+  + destruct P.
+    - inversion H2.
+    - inversion H2; subst.
+      {
+        (* decide whether P1 or P2 contains 1 which determines how to reassosciate the cut *)
+        inversion H1; subst. inversion H9; subst. inversion H8; subst.
+        inversion H11; subst.
+        + (* 1 ∈ P1 *)
+          exists (cut (down (rename_process P2 swap01))
+                  (cut (rename_process P1 swap01)
+                       (rename_process (up Q) swap01))).
+          split.
+          * eapply c_trans.
+            ** eapply c_cong_cut. eapply c_cut_comm. eapply c_refl.
+            ** eapply c_cut_assoc; auto.
+               apply ((proj1 ctx_none_not_free) _ _ 1) in H13; auto.
+          * eapply cut_list_cons.
+            ** destruct P2; simpl; try congruence.
+            ** eapply cut_list_cons.
+               *** destruct P1; simpl; try congruence.
+               *** apply renaming_preserves_cut_listness.
+                   apply upshifting_preserves_cut_listness; auto.
+        + (* 1 ∈ P2 *)
+          exists (cut (down (rename_process P1 swap01))
+                  (cut (rename_process P2 swap01)
+                       (rename_process (up Q) swap01))).
+          split.
+          * eapply c_cut_assoc; auto.
+            apply ((proj1 ctx_none_not_free) _ _ 1) in H12; auto.
+          * eapply cut_list_cons.
+            ** destruct P1; simpl; try congruence.
+            ** eapply cut_list_cons.
+               *** destruct P2; simpl; try congruence.
+               *** apply renaming_preserves_cut_listness.
+                   apply upshifting_preserves_cut_listness; auto.
+      }
+      {
+        inversion H1; subst. inversion H9; subst. inversion H8; subst.
+        inversion H11; subst.
+        + assert (
+            (cut (cut P1 P2) Q) ≡
+            (cut (down (rename_process P2 swap01))
+                  (cut (rename_process P1 swap01)
+                       (rename_process (up Q) swap01)))
+          ).
+          {
+            eapply c_trans.
+            + eapply c_cong_cut. apply c_cut_comm. apply c_refl.
+            + eapply c_cut_assoc; eauto.
+              apply ((proj1 ctx_none_not_free) _ _ 1) in H13; auto.
+          }
+
+          assert ( cut_list (down (rename_process P2 swap01)) ).
+          { apply downshift_preserves_cut_listness; apply renaming_preserves_cut_listness; auto. }
+          assert ( cut_list (cut (rename_process P1 swap01) (rename_process (up Q) swap01)) ).
+          {
+            apply cut_list_cons.
+            + destruct P1; simpl; congruence.
+            + apply renaming_preserves_cut_listness;
+              apply upshifting_preserves_cut_listness;
+              auto.
+          }
+          assert ( depth (down (rename_process P2 swap01)) <= n ).
+          {
+            unfold down.
+            rewrite <- (proj1 down_shift_preserves_depth).
+            rewrite <- (proj1 renaming_preserves_depth).
+            simpl in H; lia.
+          }
+          apply ((proj1 struct_cong_preserves_typing) _ _ H0) in H1.
+
+          destruct (IHn _ _ _ _ H15 eq_refl H1 H4 H14) as [P' [? ?]].
+          exists P'; split; auto.
+          eapply c_trans; eauto.
+        + assert (
+            (cut (cut P1 P2) Q) ≡
+            (cut (down (rename_process P1 swap01))
+                  (cut (rename_process P2 swap01)
+                       (rename_process (up Q) swap01)))
+          ).
+          {
+            eapply c_cut_assoc; auto.
+            apply ((proj1 ctx_none_not_free) _ _ 1) in H12; auto.
+          }
+
+          assert ( cut_list (rename_process P2 swap01) ).
+          { apply renaming_preserves_cut_listness; auto. }
+          assert ( cut_list (rename_process (up Q) swap01) ).
+          { apply renaming_preserves_cut_listness; apply upshifting_preserves_cut_listness; auto. }
+
+          simpl in H.
+          assert ( depth P2 <= n ) by lia.
+          assert ( depth (rename_process P2 swap01) <= n ).
+          { rewrite <- ((proj1 renaming_preserves_depth) _ swap01); auto. }
+
+          assert ( exists Γ', Γ' ⊢ cut (rename_process P2 swap01) (rename_process (up Q) swap01) :# ).
+          {
+            apply ((proj1 struct_cong_preserves_typing) _ _ H0) in H1.
+            inversion H1; subst.
+            exists (dual A1 .: Γ4); auto.
+          }
+          destruct H18 as [Γ' ?].
+
+          destruct (IHn _ _ _ _ H17 eq_refl H18 H4 H14) as [P' [? ?]].
+
+          exists (cut (down (rename_process P1 swap01)) P').
+          split.
+          - eapply c_trans; eauto.
+            eapply c_trans.
+            * eapply c_cut_comm.
+            * eapply c_trans.
+              ** eapply c_cong_cut; eauto. apply c_refl.
+              ** eapply c_cut_comm.
+          - eapply cut_list_cons; auto.
+            destruct P1; simpl; congruence.
+      }
+    - exists (cut (seq P s) Q); split.
+      * apply c_refl.
+      * eapply cut_list_cons; auto. congruence.
+    - inversion H2.
+Qed.
+
+Lemma cut_lists_flatten_in_cut :
+  forall Γ P Q,
+    Γ ⊢ (cut P Q) :# -> cut_list P -> cut_list Q ->
+    exists R, (cut P Q) ≡ R /\ cut_list R.
+Proof.
+  intros.
+  apply (cut_lists_flatten_in_cut'
+          (depth P) _ _ _ (depth P) (Nat.le_refl (depth P)) eq_refl H H0 H1).
+Qed.
+
+Lemma canonical_cut_form :
+  forall Γ L R, Γ ⊢ (cut L R) :# -> exists P', (cut L R) ≡ P' /\ cut_list P'.
+Proof.
+  intros.
+  remember (cut L R).
+  generalize dependent R.
+  generalize dependent L.
+  induction H; intros; try discriminate.
+  destruct P; destruct Q;
+  (* neither L nor R can be 'stop' if the cut is well-typed *)
+  try ( match goal with [ H : (?A .: ?Γ) ⊢ stop :# |- _ ] => inversion H; ctx_eq_contra end );
+  (* if both L and R are no cuts, then argue by reflexivity *)
+  try now (
+    match goal with
+    | [ Heq : cut ?X ?Y = cut L R |- _ ] =>
+      exists (cut X Y); split; try apply c_refl; try econstructor; try congruence
+    end
+  ).
+  + specialize IHTypingP2 with Q1 Q2.
+    destruct (IHTypingP2 eq_refl) as [P'' [? ?]].
+    exists (cut (link m m0) P''); split.
+    - eapply c_trans.
+      * eapply c_cut_comm.
+      * eapply c_trans.
+        ** eapply c_cong_cut.
+           *** eassumption.
+           *** apply c_refl.
+        ** eapply c_cut_comm.
+    - eapply cut_list_cons; eauto. congruence.
+  + specialize IHTypingP1 with P1 P2.
+    destruct (IHTypingP1 eq_refl) as [P'' [? ?]].
+    exists (cut (link m m0) P''); split.
+    - eapply c_trans.
+      * eapply c_cong_cut; eauto. eapply c_refl.
+      * eapply c_cut_comm.
+    - eapply cut_list_cons; eauto. congruence.
+  + (* both operands of the cut are themselves cut lists and may be flattened into one *)
+    specialize IHTypingP1 with P1 P2. destruct (IHTypingP1 eq_refl) as [P'' [? ?]].
+    specialize IHTypingP2 with Q1 Q2. destruct (IHTypingP2 eq_refl) as [Q'' [? ?]].
+    assert ( Γ ⊢ cut P'' Q'' :# ).
+    {
+      econstructor; eauto.
+      + apply ((proj1 struct_cong_preserves_typing) _ _ H2 _); eauto.
+      + apply ((proj1 struct_cong_preserves_typing) _ _ H4 _); eauto.
+    }
+    destruct (cut_lists_flatten_in_cut _ _ _ H6 H3 H5) as [R' [? ?]].
+    exists R'; split; auto.
+    eapply c_trans.
+    - eapply c_cong_cut; eauto.
+    - eauto.
+  + specialize IHTypingP1 with P1 P2.
+    destruct (IHTypingP1 eq_refl) as [P'' [? ?]].
+    exists (cut (seq Q s) P''); split.
+    - eapply c_trans.
+      * eapply c_cong_cut; eauto. eapply c_refl.
+      * eapply c_cut_comm.
+    - eapply cut_list_cons; eauto. congruence.
+  + specialize IHTypingP2 with Q1 Q2.
+    destruct (IHTypingP2 eq_refl) as [P'' [? ?]].
+    exists (cut (seq P s) P''); split.
+    - eapply c_trans.
+      * eapply c_cut_comm.
+      * eapply c_trans.
+        ** eapply c_cong_cut.
+           *** eassumption.
+           *** apply c_refl.
+        ** eapply c_cut_comm.
+    - eapply cut_list_cons; eauto. congruence.
+Qed.
+
+(******************************************************************************)
+(* Properties about link processes                                            *)
+(******************************************************************************)
+Lemma link_reduces_or_contains_future :
+  forall Γ M1 M2, Γ ⊢ (link M1 M2) :# ->
+    (exists P', (link M1 M2) ⊳ P') \/
+    (exists i, M1 = future i \/ M2 = future i).
+Proof.
+  intros.
+  destruct M1; destruct M2; inversion H; subst.
+  + right. exists n. left; reflexivity.
+  + right. exists n. left; reflexivity.
+  + right. exists n. right; reflexivity.
+  + left.
+    inversion H4; inversion H5; subst.
+    inversion H3; inversion H9; subst;
+    simpl in *; try discriminate.
+    (* well-typed logical redex reduce according to their corresponding beta rule *)
+    * exists (cut Q Q1); econstructor.
+    * exists (cut Q Q2); econstructor.
+    * exists (cut Q Q1).
+      eapply r_struct with (P' := link (prefix (choose_left Q)) (prefix (offer_choice Q1 Q2))).
+      ** eapply c_link.
+      ** econstructor.
+      ** apply c_refl.
+    * exists (cut Q Q2).
+      eapply r_struct with (P' := link (prefix (choose_right Q)) (prefix (offer_choice Q1 Q2))).
+      ** eapply c_link.
+      ** econstructor.
+      ** apply c_refl.
+    * exists (cut (cut Q0 (rename_process (up Q) swap01)) R); econstructor; eauto.
+    * exists (cut (cut Q (rename_process (up Q0) swap01)) R).
+      eapply r_struct with (P' := link (prefix (send Q0 R)) (prefix (receive Q))).
+      ** eapply c_link.
+      ** econstructor. reflexivity.
+      ** apply c_refl.
+    * exists Q; econstructor.
+    * exists Q. eapply r_struct with (P' := link (prefix close) (prefix (wait Q))).
+      ** eapply c_link.
+      ** econstructor.
+      ** apply c_refl.
+Qed.
+
+Corollary link_final_or_reduces :
+  forall Γ M1 M2, Γ ⊢ (link M1 M2) :# ->
+    final (link M1 M2) \/ (exists P', (link M1 M2) ⊳ P').
+Proof.
+  intros. destruct (link_reduces_or_contains_future _ _ _ H).
+  + right; auto.
+  + left. destruct H0 as [i [? | ?]]; subst; econstructor.
+Qed.
+
+(******************************************************************************)
+(* Relation between Cut List and Link List                                    *)
+(******************************************************************************)
+(* useful lemmas for below
+   if x in xs and x > 0 and link_list xs P then pred x free in P
+*)
+Lemma link_list_with_0_at_0_reduces :
+  forall P xs,
+    link_list (0 :: xs) P -> exists Q, P ⊳ Q.
+Proof.
+  intros P xs H. inversion H;
+  try match goal with
+  | [ H : cut (link (future 0) ?M1) ?P2 = P |- _ ]
+      => exists (subst_process P2 ((downM M1) ⋅ id_subst)); econstructor; eauto
+  | [ H : cut (link ?M1 (future 0)) ?P2 = P |- _ ]
+      => exists (subst_process P2 ((downM M1) ⋅ id_subst));
+         econstructor; [ eapply c_cong_cut; [eapply c_link | eapply c_refl] | econstructor | apply c_refl ]
+  end.
+Qed.
+
+Local Hint Rewrite
+  swap_swap_id
+  down_after_up_process_id
+  up_after_down_process_id
+    : up_down_rename_rewrites.
+
+Lemma link_list_with_0_at_1_reduces :
+  forall Γ P xs n0,
+    Γ ⊢ P :# -> link_list (n0 :: 0 :: xs) P -> exists Q, P ⊳ Q.
+Proof.
+  intros. inversion H0; subst;
+  try match goal with
+    | [ H : _ ⊢ cut ?P1 (link (future 0) ?M) :# |- _]
+        => exists (subst_process P1 ((downM M) ⋅ id_subst));
+           eapply r_struct; [ eapply c_cut_comm | econstructor | apply c_refl]
+    | [ H : _ ⊢ cut ?P1 (link ?M (future 0)) :# |- _]
+        => exists (subst_process P1 ((downM M) ⋅ id_subst));
+           eapply r_struct;
+           [eapply c_trans; [eapply c_cut_comm | eapply c_cong_cut; [eapply c_link | eapply c_refl]]
+                             | econstructor | apply c_refl ]
+    end;
+  simpl in H4; inversion H4; subst;
+  try match goal with
+    | [ H   : link_list _ (cut ?L ((cut (link (future 1) ?M)) ?P)),
+        Hwt : _ ⊢ (cut ?L ((cut (link (future 1) ?M)) ?P)) :#
+        |- _ ]
+      => eexists; eapply r_struct;
+          [
+            eapply c_comm; eapply (c_cut_assoc
+              (rename_process (up L) swap01)
+              (rename_process (link (future 1) M) swap01)
+              (down (rename_process P swap01))
+            ); autorewrite with up_down_rename_rewrites; auto;
+            [ apply nfv_10_swap; apply nfv_lift_n; lia
+            | apply nfv_01_swap; intro Hfv; inversion Hwt; subst;
+              match goal with
+              | [ Hwt1 : _ ⊢ cut (link (future 1) ?M) ?P :# |- _ ]
+                => inversion Hwt1; subst;
+                   match goal with
+                   | [ HwtM : (_ .: ?Γ1) ⊢ link (future 1) M :#,
+                       HwtP : (_ .: ?Γ2) ⊢ P :#,
+                       Hsplit : _ ≜ ?Γ1 ∘ ?Γ2
+                       |- _ ]
+                      => inversion Hsplit; subst;
+                         assert (1 ∈ (link (future 1) M)) as Hfv1link by repeat econstructor;
+                         destruct ((proj1 free_vars_decidable) P 1); auto;
+                         apply ((proj1 free_var_in_ctx) _ _ Hfv1link) in HwtM;
+                         apply ((proj1 free_var_in_ctx) _ _ H1) in HwtP;
+                         destruct HwtM, HwtP; simpl in *; subst;
+                         match goal with
+                         | [ Hsplitentry : split_entry _ _ _ |- _ ] => inversion Hsplitentry
+                         end
+                   end
+              end
+            ]
+          | eapply r_cong_cut; eapply r_struct;
+            [ apply c_cut_comm | simpl; econstructor | eapply c_refl ]
+          | eapply c_refl
+          ]
+    end;
+  try match goal with
+    | [ H   : link_list _ (cut ?L ((cut (link ?M (future 1))) ?P)),
+        Hwt : _ ⊢ (cut ?L ((cut (link ?M (future 1))) ?P)) :#
+        |- _ ]
+      => eexists ; eapply r_struct;
+          [
+            eapply c_comm; eapply (c_cut_assoc
+              (rename_process (up L) swap01)
+              (rename_process (link M (future 1)) swap01)
+              (down (rename_process P swap01))
+            ); autorewrite with up_down_rename_rewrites; auto;
+            [ apply nfv_10_swap; apply nfv_lift_n; lia
+            | apply nfv_01_swap; intro Hfv; inversion Hwt; subst;
+              match goal with
+              | [ Hwt1 : _ ⊢ cut (link ?M (future 1)) ?P :# |- _ ]
+                => inversion Hwt1; subst;
+                   match goal with
+                   | [ HwtM : (_ .: ?Γ1) ⊢ link M (future 1) :#,
+                       HwtP : (_ .: ?Γ2) ⊢ P :#,
+                       Hsplit : _ ≜ ?Γ1 ∘ ?Γ2
+                       |- _ ]
+                      => inversion Hsplit; subst;
+                         assert (1 ∈ (link M (future 1))) as Hfv1link by repeat econstructor;
+                         destruct ((proj1 free_vars_decidable) P 1); auto;
+                         apply ((proj1 free_var_in_ctx) _ _ Hfv1link) in HwtM;
+                         apply ((proj1 free_var_in_ctx) _ _ H1) in HwtP;
+                         destruct HwtM, HwtP; simpl in *; subst;
+                         match goal with
+                         | [ Hsplitentry : split_entry _ _ _ |- _ ] => inversion Hsplitentry
+                         end
+                   end
+              end
+            ]
+          | eapply r_cong_cut; eapply r_struct;
+            [ eapply c_trans; [ eapply c_cut_comm | eapply c_cong_cut; simpl; apply c_link; eapply c_refl ]
+            | simpl; econstructor
+            | eapply c_refl ]
+          | eapply c_refl
+          ]
+    end.
+Qed.
+
+Lemma link_list_rename :
+  forall P xs r,
+    (forall x, List.In x xs -> x > 0) ->
+    bijective r -> link_list xs P -> link_list (List.map S (List.map r (List.map Nat.pred xs))) (rename_process P r).
+Proof.
+  intros.
+  generalize dependent r.
+  induction H1; intros;
+  try destruct i1, i2; try (specialize H with 0; simpl in H; exfalso; lia); try (simpl; econstructor).
+  + destruct i; try (specialize H with 0; simpl in H; exfalso; lia).
+    simpl. econstructor.
+    assert (bijective (up_ren r)). { apply shift_preserves_bijection; auto. }
+    assert (forall x : nat, List.In x (ListDef.map S xs) -> x > 0).
+    { intros. apply List.in_map_iff in H3. destruct H3 as [x0 []]. lia. }
+    pose proof (IHlink_list H3 _ H2).
+    clear - H H4.
+    repeat rewrite List.map_map in *.
+    assert (
+      ListDef.map (fun x : nat => S (up_ren r (Nat.pred (S x)))) xs
+        = ListDef.map (fun x : nat => S (S (r (Nat.pred x)))) xs
+    ).
+    {
+      apply List.map_ext_in. intros. specialize H with a.
+      simpl in H. assert (S i = a \/ List.In a xs) by auto.
+      apply H in H1. destruct a; auto. exfalso; lia.
+    }
+    rewrite <- H0. auto.
+  + destruct i; try (specialize H with 0; simpl in H; exfalso; lia).
+    simpl. econstructor.
+    assert (bijective (up_ren r)). { apply shift_preserves_bijection; auto. }
+    assert (forall x : nat, List.In x (ListDef.map S xs) -> x > 0).
+    { intros. apply List.in_map_iff in H3. destruct H3 as [x0 []]. lia. }
+    pose proof (IHlink_list H3 _ H2).
+    clear - H H4.
+    repeat rewrite List.map_map in *.
+    assert (
+      ListDef.map (fun x : nat => S (up_ren r (Nat.pred (S x)))) xs
+        = ListDef.map (fun x : nat => S (S (r (Nat.pred x)))) xs
+    ).
+    {
+      apply List.map_ext_in. intros. specialize H with a.
+      simpl in H. assert (S i = a \/ List.In a xs) by auto.
+      apply H in H1. destruct a; auto. exfalso; lia.
+    }
+    rewrite <- H0. auto.
+Qed.
+
+Lemma link_list_free_vars :
+  forall P xs,
+    (forall x, List.In x xs -> x > 0) ->
+    link_list xs P ->
+    (forall x, List.In x xs -> (Nat.pred x) ∈ P).
+Proof.
+  intros.
+  generalize dependent x.
+  induction H0; intros.
+  + simpl in H1. destruct H1; subst.
+    - apply fv_cut_l. simpl in H; specialize H with x.
+      replace (S (Nat.pred x)) with x by lia.
+      repeat econstructor.
+    - destruct H0; try contradiction; subst.
+      apply fv_cut_r; simpl in H; specialize H with x.
+      replace (S (Nat.pred x)) with x by lia.
+      repeat econstructor.
+  + simpl in H1. destruct H1; subst.
+    - apply fv_cut_l. simpl in H; specialize H with x.
+      replace (S (Nat.pred x)) with x by lia.
+      repeat econstructor.
+    - destruct H0; try contradiction; subst.
+      apply fv_cut_r; simpl in H; specialize H with x.
+      replace (S (Nat.pred x)) with x by lia.
+      apply fv_link_r; econstructor.
+  + simpl in H1. destruct H1; subst.
+    - apply fv_cut_l. simpl in H; specialize H with x.
+      replace (S (Nat.pred x)) with x by lia.
+      apply fv_link_r; econstructor.
+    - destruct H0; try contradiction; subst.
+      apply fv_cut_r; simpl in H; specialize H with x.
+      replace (S (Nat.pred x)) with x by lia.
+      repeat econstructor.
+  + simpl in H1. destruct H1; subst.
+    - apply fv_cut_l. simpl in H; specialize H with x.
+      replace (S (Nat.pred x)) with x by lia.
+      apply fv_link_r; econstructor.
+    - destruct H0; try contradiction; subst.
+      apply fv_cut_r; simpl in H; specialize H with x.
+      replace (S (Nat.pred x)) with x by lia.
+      apply fv_link_r; econstructor.
+  + simpl in H1. destruct H1; subst.
+    - apply fv_cut_l. specialize H with x.
+      simpl in H. replace (S (Nat.pred x)) with x by lia.
+      repeat econstructor.
+    - apply fv_cut_r. simpl in H. specialize H with x.
+      pose proof (H (or_intror H1)).
+      replace (S (Nat.pred x)) with x by lia.
+      assert (forall x : nat, List.In x (ListDef.map S xs) -> x > 0).
+      { intros. apply List.in_map_iff in H3; destruct H3. lia. }
+      apply (IHlink_list H3 (S x)).
+      apply List.in_map_iff. exists x; auto.
+  + simpl in H1. destruct H1; subst.
+    - apply fv_cut_l. specialize H with x.
+      simpl in H. replace (S (Nat.pred x)) with x by lia.
+      apply fv_link_r. econstructor.
+    - apply fv_cut_r. simpl in H. specialize H with x.
+      pose proof (H (or_intror H1)).
+      replace (S (Nat.pred x)) with x by lia.
+      assert (forall x : nat, List.In x (ListDef.map S xs) -> x > 0).
+      { intros. apply List.in_map_iff in H3; destruct H3. lia. }
+      eapply (IHlink_list H3 (S x)).
+      apply List.in_map_iff. exists x; auto.
+Qed.
+
+Lemma link_list_swap_0_1 :
+  forall Γ P n0 n1 xs,
+    0 <> n0 ->
+    0 <> n1 ->
+    Γ ⊢ P :# -> List.In 0 xs -> link_list (n0 :: n1 :: xs) P ->
+    exists Q Q' xs', P ≡ (cut Q Q') /\ link_list xs' Q' /\ List.In 0 xs' /\ length xs' <= S (length xs).
+Proof.
+  intros.
+  inversion H3; subst; try now inversion H2.
+  + simpl in H7. inversion H7; subst.
+    - assert (xs = [0]).
+      {
+        destruct xs.
+        + simpl in H6; congruence.
+        + destruct xs.
+          - simpl in H6. simpl in H2. destruct H2.
+            * subst. auto.
+            * contradiction.
+          - simpl in H6. inversion H6.
+      }
+      assert (i2 = 1).
+      { rewrite H4 in H6. inversion H6; subst; auto. }
+      subst.
+      eexists; eexists. exists [S n0; 0].
+      repeat split.
+      * eapply c_trans.
+        ** eapply c_cong_cut; [ eapply c_refl | eapply c_cut_comm ].
+        ** eapply c_trans.
+           *** eapply c_comm. eapply (c_cut_assoc
+                (rename_process (up (link (future n0) M)) swap01)
+                (rename_process (link (future 1) M2) swap01)
+                (down (rename_process (link (future (S n1)) M1) swap01))
+               ); autorewrite with up_down_rename_rewrites; auto;
+                [ apply nfv_10_swap; apply nfv_lift_n; lia
+                | apply nfv_01_swap; intro Hfv; inversion H1; subst
+                ].
+                assert (1 ∈ (link (future 1) M2)) as Hfv1link by repeat econstructor.
+                inversion H11; subst. inversion H9; subst.
+                apply ((proj1 free_var_in_ctx) _ _ Hfv) in H13.
+                apply ((proj1 free_var_in_ctx) _ _ Hfv1link) in H14.
+                destruct H13, H14; simpl in *; subst. inversion H9. inversion H14.
+           *** eapply c_cut_comm.
+      * simpl. destruct n0; try congruence. econstructor.
+      * simpl. right; left; auto.
+      * simpl; lia.
+    - assert (xs = [0]).
+      {
+        destruct xs.
+        + simpl in H6; congruence.
+        + destruct xs.
+          - simpl in H6. simpl in H2. destruct H2.
+            * subst. auto.
+            * contradiction.
+          - simpl in H6. inversion H6.
+      }
+      assert (i2 = 1).
+      { rewrite H4 in H6. inversion H6; subst; auto. }
+      subst.
+      eexists; eexists. exists [S n0; 0].
+      repeat split.
+      * eapply c_trans.
+        ** eapply c_cong_cut; [ eapply c_refl | eapply c_cut_comm ].
+        ** eapply c_trans.
+           *** eapply c_comm. eapply (c_cut_assoc
+                (rename_process (up (link (future n0) M)) swap01)
+                (rename_process (link M2 (future 1)) swap01)
+                (down (rename_process (link (future (S n1)) M1) swap01))
+               ); autorewrite with up_down_rename_rewrites; auto;
+                [ apply nfv_10_swap; apply nfv_lift_n; lia
+                | apply nfv_01_swap; intro Hfv; inversion H1; subst
+                ].
+                assert (1 ∈ (link M2 (future 1))) as Hfv1link by repeat econstructor.
+                inversion H11; subst. inversion H9; subst.
+                apply ((proj1 free_var_in_ctx) _ _ Hfv) in H13.
+                apply ((proj1 free_var_in_ctx) _ _ Hfv1link) in H14.
+                destruct H13, H14; simpl in *; subst. inversion H9. inversion H14.
+           *** eapply c_cut_comm.
+      * simpl. destruct n0; try congruence. econstructor.
+      * simpl. right; left; auto.
+      * simpl; lia.
+    - assert (xs = [0]).
+      {
+        destruct xs.
+        + simpl in H6; congruence.
+        + destruct xs.
+          - simpl in H6. simpl in H2. destruct H2.
+            * subst. auto.
+            * contradiction.
+          - simpl in H6. inversion H6.
+      }
+      assert (i2 = 1).
+      { rewrite H4 in H6. inversion H6; subst; auto. }
+      subst.
+      eexists; eexists. exists [S n0; 0].
+      repeat split.
+      * eapply c_trans.
+        ** eapply c_cong_cut; [ eapply c_refl | eapply c_cut_comm ].
+        ** eapply c_trans.
+           *** eapply c_comm. eapply (c_cut_assoc
+                (rename_process (up (link (future n0) M)) swap01)
+                (rename_process (link (future 1) M2) swap01)
+                (down (rename_process (link M1 (future (S n1))) swap01))
+               ); autorewrite with up_down_rename_rewrites; auto;
+                [ apply nfv_10_swap; apply nfv_lift_n; lia
+                | apply nfv_01_swap; intro Hfv; inversion H1; subst
+                ].
+                assert (1 ∈ (link (future 1) M2)) as Hfv1link by repeat econstructor.
+                inversion H11; subst. inversion H9; subst.
+                apply ((proj1 free_var_in_ctx) _ _ Hfv) in H13.
+                apply ((proj1 free_var_in_ctx) _ _ Hfv1link) in H14.
+                destruct H13, H14; simpl in *; subst. inversion H9. inversion H14.
+           *** eapply c_cut_comm.
+      * simpl. destruct n0; try congruence. econstructor.
+      * simpl. right; left; auto.
+      * simpl; lia.
+    - assert (xs = [0]).
+      {
+        destruct xs.
+        + simpl in H6; congruence.
+        + destruct xs.
+          - simpl in H6. simpl in H2. destruct H2.
+            * subst. auto.
+            * contradiction.
+          - simpl in H6. inversion H6.
+      }
+      assert (i2 = 1).
+      { rewrite H4 in H6. inversion H6; subst; auto. }
+      subst.
+      eexists; eexists. exists [S n0; 0].
+      repeat split.
+      * eapply c_trans.
+        ** eapply c_cong_cut; [ eapply c_refl | eapply c_cut_comm ].
+        ** eapply c_trans.
+           *** eapply c_comm. eapply (c_cut_assoc
+                (rename_process (up (link (future n0) M)) swap01)
+                (rename_process (link M2 (future 1)) swap01)
+                (down (rename_process (link M1 (future (S n1))) swap01))
+               ); autorewrite with up_down_rename_rewrites; auto;
+                [ apply nfv_10_swap; apply nfv_lift_n; lia
+                | apply nfv_01_swap; intro Hfv; inversion H1; subst
+                ].
+                assert (1 ∈ (link M2 (future 1))) as Hfv1link by repeat econstructor.
+                inversion H11; subst. inversion H9; subst.
+                apply ((proj1 free_var_in_ctx) _ _ Hfv) in H13.
+                apply ((proj1 free_var_in_ctx) _ _ Hfv1link) in H14.
+                destruct H13, H14; simpl in *; subst. inversion H9. inversion H14.
+           *** eapply c_cut_comm.
+      * simpl. destruct n0; try congruence. econstructor.
+      * simpl. right; left; auto.
+      * simpl; lia.
+    - assert (forall x, List.In x (List.map S (List.map S xs)) -> x > 0).
+      { intros. apply List.in_map_iff in H4; destruct H4. lia. }
+      pose proof (link_list_rename _ _ _ H4 swap01_is_bijective H8).
+      rewrite (List.map_map S Nat.pred _) in H5.
+      simpl in H5.
+      rewrite List.map_id in H5.
+      eexists; eexists.
+      exists ((S n0) :: (List.map swap01 (List.map S xs))).
+      repeat split.
+      * eapply c_trans.
+        ** eapply c_cong_cut; [ eapply c_refl | eapply c_cut_comm ].
+        ** eapply c_trans.
+           *** eapply c_comm. eapply (c_cut_assoc
+                (rename_process (up (link (future n0) M)) swap01)
+                (rename_process P swap01)
+                (down (rename_process (link (future (S n1)) M0) swap01))
+               ); autorewrite with up_down_rename_rewrites; auto;
+                [ apply nfv_10_swap; apply nfv_lift_n; lia
+                | apply nfv_01_swap; intro Hfv; inversion H1; subst
+                ].
+                assert (1 ∈ P).
+                {
+                  replace 1 with (Nat.pred 2) by auto.
+                  assert (List.In 2 (List.map S (List.map S xs))).
+                  { rewrite List.map_map. apply List.in_map_iff. exists 0; auto. }
+                  apply (link_list_free_vars _ _ H4 H8 2 H6).
+                }
+                inversion H13; subst. inversion H14; subst.
+                destruct ((proj1 free_vars_decidable) (link (future (S n1)) M0) 1); auto.
+                apply ((proj1 free_var_in_ctx) _ _ Hfv) in H16.
+                apply ((proj1 free_var_in_ctx) _ _ H6) in H17.
+                destruct H16, H17; simpl in *; subst. inversion H14. inversion H18.
+           *** eapply c_cut_comm.
+      * destruct n0; try congruence. simpl. unfold relocate. simpl.
+        econstructor; eauto.
+      * simpl. right.
+        rewrite List.map_map.
+        apply List.in_map_iff. exists 0; split; auto.
+      * simpl. repeat rewrite List.length_map. lia.
+    - assert (forall x, List.In x (List.map S (List.map S xs)) -> x > 0).
+      { intros. apply List.in_map_iff in H4; destruct H4. lia. }
+      pose proof (link_list_rename _ _ _ H4 swap01_is_bijective H8).
+      rewrite (List.map_map S Nat.pred _) in H5.
+      simpl in H5.
+      rewrite List.map_id in H5.
+      eexists; eexists.
+      exists ((S n0) :: (List.map swap01 (List.map S xs))).
+      repeat split.
+      * eapply c_trans.
+        ** eapply c_cong_cut; [ eapply c_refl | eapply c_cut_comm ].
+        ** eapply c_trans.
+           *** eapply c_comm. eapply (c_cut_assoc
+                (rename_process (up (link (future n0) M)) swap01)
+                (rename_process P swap01)
+                (down (rename_process (link M0 (future (S n1))) swap01))
+               ); autorewrite with up_down_rename_rewrites; auto;
+                [ apply nfv_10_swap; apply nfv_lift_n; lia
+                | apply nfv_01_swap; intro Hfv; inversion H1; subst
+                ].
+                assert (1 ∈ P).
+                {
+                  replace 1 with (Nat.pred 2) by auto.
+                  assert (List.In 2 (List.map S (List.map S xs))).
+                  { rewrite List.map_map. apply List.in_map_iff. exists 0; auto. }
+                  apply (link_list_free_vars _ _ H4 H8 2 H6).
+                }
+                inversion H13; subst. inversion H14; subst.
+                destruct ((proj1 free_vars_decidable) (link M0 (future (S n1))) 1); auto.
+                apply ((proj1 free_var_in_ctx) _ _ Hfv) in H16.
+                apply ((proj1 free_var_in_ctx) _ _ H6) in H17.
+                destruct H16, H17; simpl in *; subst. inversion H14. inversion H18.
+           *** eapply c_cut_comm.
+      * destruct n0; try congruence. simpl. unfold relocate. simpl.
+        econstructor; eauto.
+      * simpl. right.
+        rewrite List.map_map.
+        apply List.in_map_iff. exists 0; split; auto.
+      * simpl. repeat rewrite List.length_map. lia.
+  + simpl in H7. inversion H7; subst.
+    - assert (xs = [0]).
+      {
+        destruct xs.
+        + simpl in H6; congruence.
+        + destruct xs.
+          - simpl in H6. simpl in H2. destruct H2.
+            * subst. auto.
+            * contradiction.
+          - simpl in H6. inversion H6.
+      }
+      assert (i2 = 1).
+      { rewrite H4 in H6. inversion H6; subst; auto. }
+      subst.
+      eexists; eexists. exists [S n0; 0].
+      repeat split.
+      * eapply c_trans.
+        ** eapply c_cong_cut; [ eapply c_refl | eapply c_cut_comm ].
+        ** eapply c_trans.
+           *** eapply c_comm. eapply (c_cut_assoc
+                (rename_process (up (link M (future n0))) swap01)
+                (rename_process (link (future 1) M2) swap01)
+                (down (rename_process (link (future (S n1)) M1) swap01))
+               ); autorewrite with up_down_rename_rewrites; auto;
+                [ apply nfv_10_swap; apply nfv_lift_n; lia
+                | apply nfv_01_swap; intro Hfv; inversion H1; subst
+                ].
+                assert (1 ∈ (link (future 1) M2)) as Hfv1link by repeat econstructor.
+                inversion H11; subst. inversion H9; subst.
+                apply ((proj1 free_var_in_ctx) _ _ Hfv) in H13.
+                apply ((proj1 free_var_in_ctx) _ _ Hfv1link) in H14.
+                destruct H13, H14; simpl in *; subst. inversion H9. inversion H14.
+           *** eapply c_cut_comm.
+      * simpl. destruct n0; try congruence. econstructor.
+      * simpl. right; left; auto.
+      * simpl; lia.
+    - assert (xs = [0]).
+      {
+        destruct xs.
+        + simpl in H6; congruence.
+        + destruct xs.
+          - simpl in H6. simpl in H2. destruct H2.
+            * subst. auto.
+            * contradiction.
+          - simpl in H6. inversion H6.
+      }
+      assert (i2 = 1).
+      { rewrite H4 in H6. inversion H6; subst; auto. }
+      subst.
+      eexists; eexists. exists [S n0; 0].
+      repeat split.
+      * eapply c_trans.
+        ** eapply c_cong_cut; [ eapply c_refl | eapply c_cut_comm ].
+        ** eapply c_trans.
+           *** eapply c_comm. eapply (c_cut_assoc
+                (rename_process (up (link M (future n0))) swap01)
+                (rename_process (link M2 (future 1)) swap01)
+                (down (rename_process (link (future (S n1)) M1) swap01))
+               ); autorewrite with up_down_rename_rewrites; auto;
+                [ apply nfv_10_swap; apply nfv_lift_n; lia
+                | apply nfv_01_swap; intro Hfv; inversion H1; subst
+                ].
+                assert (1 ∈ (link M2 (future 1))) as Hfv1link by repeat econstructor.
+                inversion H11; subst. inversion H9; subst.
+                apply ((proj1 free_var_in_ctx) _ _ Hfv) in H13.
+                apply ((proj1 free_var_in_ctx) _ _ Hfv1link) in H14.
+                destruct H13, H14; simpl in *; subst. inversion H9. inversion H14.
+           *** eapply c_cut_comm.
+      * simpl. destruct n0; try congruence. econstructor.
+      * simpl. right; left; auto.
+      * simpl; lia.
+    - assert (xs = [0]).
+      {
+        destruct xs.
+        + simpl in H6; congruence.
+        + destruct xs.
+          - simpl in H6. simpl in H2. destruct H2.
+            * subst. auto.
+            * contradiction.
+          - simpl in H6. inversion H6.
+      }
+      assert (i2 = 1).
+      { rewrite H4 in H6. inversion H6; subst; auto. }
+      subst.
+      eexists; eexists. exists [S n0; 0].
+      repeat split.
+      * eapply c_trans.
+        ** eapply c_cong_cut; [ eapply c_refl | eapply c_cut_comm ].
+        ** eapply c_trans.
+           *** eapply c_comm. eapply (c_cut_assoc
+                (rename_process (up (link M (future n0))) swap01)
+                (rename_process (link (future 1) M2) swap01)
+                (down (rename_process (link M1 (future (S n1))) swap01))
+               ); autorewrite with up_down_rename_rewrites; auto;
+                [ apply nfv_10_swap; apply nfv_lift_n; lia
+                | apply nfv_01_swap; intro Hfv; inversion H1; subst
+                ].
+                assert (1 ∈ (link (future 1) M2)) as Hfv1link by repeat econstructor.
+                inversion H11; subst. inversion H9; subst.
+                apply ((proj1 free_var_in_ctx) _ _ Hfv) in H13.
+                apply ((proj1 free_var_in_ctx) _ _ Hfv1link) in H14.
+                destruct H13, H14; simpl in *; subst. inversion H9. inversion H14.
+           *** eapply c_cut_comm.
+      * simpl. destruct n0; try congruence. econstructor.
+      * simpl. right; left; auto.
+      * simpl; lia.
+    - assert (xs = [0]).
+      {
+        destruct xs.
+        + simpl in H6; congruence.
+        + destruct xs.
+          - simpl in H6. simpl in H2. destruct H2.
+            * subst. auto.
+            * contradiction.
+          - simpl in H6. inversion H6.
+      }
+      assert (i2 = 1).
+      { rewrite H4 in H6. inversion H6; subst; auto. }
+      subst.
+      eexists; eexists. exists [S n0; 0].
+      repeat split.
+      * eapply c_trans.
+        ** eapply c_cong_cut; [ eapply c_refl | eapply c_cut_comm ].
+        ** eapply c_trans.
+           *** eapply c_comm. eapply (c_cut_assoc
+                (rename_process (up (link M (future n0))) swap01)
+                (rename_process (link M2 (future 1)) swap01)
+                (down (rename_process (link M1 (future (S n1))) swap01))
+               ); autorewrite with up_down_rename_rewrites; auto;
+                [ apply nfv_10_swap; apply nfv_lift_n; lia
+                | apply nfv_01_swap; intro Hfv; inversion H1; subst
+                ].
+                assert (1 ∈ (link M2 (future 1))) as Hfv1link by repeat econstructor.
+                inversion H11; subst. inversion H9; subst.
+                apply ((proj1 free_var_in_ctx) _ _ Hfv) in H13.
+                apply ((proj1 free_var_in_ctx) _ _ Hfv1link) in H14.
+                destruct H13, H14; simpl in *; subst. inversion H9. inversion H14.
+           *** eapply c_cut_comm.
+      * simpl. destruct n0; try congruence. econstructor.
+      * simpl. right; left; auto.
+      * simpl; lia.
+    - assert (forall x, List.In x (List.map S (List.map S xs)) -> x > 0).
+      { intros. apply List.in_map_iff in H4; destruct H4. lia. }
+      pose proof (link_list_rename _ _ _ H4 swap01_is_bijective H8).
+      rewrite (List.map_map S Nat.pred _) in H5.
+      simpl in H5.
+      rewrite List.map_id in H5.
+      eexists; eexists.
+      exists ((S n0) :: (List.map swap01 (List.map S xs))).
+      repeat split.
+      * eapply c_trans.
+        ** eapply c_cong_cut; [ eapply c_refl | eapply c_cut_comm ].
+        ** eapply c_trans.
+           *** eapply c_comm. eapply (c_cut_assoc
+                (rename_process (up (link M (future n0))) swap01)
+                (rename_process P swap01)
+                (down (rename_process (link (future (S n1)) M0) swap01))
+               ); autorewrite with up_down_rename_rewrites; auto;
+                [ apply nfv_10_swap; apply nfv_lift_n; lia
+                | apply nfv_01_swap; intro Hfv; inversion H1; subst
+                ].
+                assert (1 ∈ P).
+                {
+                  replace 1 with (Nat.pred 2) by auto.
+                  assert (List.In 2 (List.map S (List.map S xs))).
+                  { rewrite List.map_map. apply List.in_map_iff. exists 0; auto. }
+                  apply (link_list_free_vars _ _ H4 H8 2 H6).
+                }
+                inversion H13; subst. inversion H14; subst.
+                destruct ((proj1 free_vars_decidable) (link (future (S n1)) M0) 1); auto.
+                apply ((proj1 free_var_in_ctx) _ _ Hfv) in H16.
+                apply ((proj1 free_var_in_ctx) _ _ H6) in H17.
+                destruct H16, H17; simpl in *; subst. inversion H14. inversion H18.
+           *** eapply c_cut_comm.
+      * destruct n0; try congruence. simpl. unfold relocate. simpl.
+        econstructor; eauto.
+      * simpl. right.
+        rewrite List.map_map.
+        apply List.in_map_iff. exists 0; split; auto.
+      * simpl. repeat rewrite List.length_map. lia.
+    - assert (forall x, List.In x (List.map S (List.map S xs)) -> x > 0).
+      { intros. apply List.in_map_iff in H4; destruct H4. lia. }
+      pose proof (link_list_rename _ _ _ H4 swap01_is_bijective H8).
+      rewrite (List.map_map S Nat.pred _) in H5.
+      simpl in H5.
+      rewrite List.map_id in H5.
+      eexists; eexists.
+      exists ((S n0) :: (List.map swap01 (List.map S xs))).
+      repeat split.
+      * eapply c_trans.
+        ** eapply c_cong_cut; [ eapply c_refl | eapply c_cut_comm ].
+        ** eapply c_trans.
+           *** eapply c_comm. eapply (c_cut_assoc
+                (rename_process (up (link M (future n0))) swap01)
+                (rename_process P swap01)
+                (down (rename_process (link M0 (future (S n1))) swap01))
+               ); autorewrite with up_down_rename_rewrites; auto;
+                [ apply nfv_10_swap; apply nfv_lift_n; lia
+                | apply nfv_01_swap; intro Hfv; inversion H1; subst
+                ].
+                assert (1 ∈ P).
+                {
+                  replace 1 with (Nat.pred 2) by auto.
+                  assert (List.In 2 (List.map S (List.map S xs))).
+                  { rewrite List.map_map. apply List.in_map_iff. exists 0; auto. }
+                  apply (link_list_free_vars _ _ H4 H8 2 H6).
+                }
+                inversion H13; subst. inversion H14; subst.
+                destruct ((proj1 free_vars_decidable) (link M0 (future (S n1))) 1); auto.
+                apply ((proj1 free_var_in_ctx) _ _ Hfv) in H16.
+                apply ((proj1 free_var_in_ctx) _ _ H6) in H17.
+                destruct H16, H17; simpl in *; subst. inversion H14. inversion H18.
+           *** eapply c_cut_comm.
+      * destruct n0; try congruence. simpl. unfold relocate. simpl.
+        econstructor; eauto.
+      * simpl. right.
+        rewrite List.map_map.
+        apply List.in_map_iff. exists 0; split; auto.
+      * simpl. repeat rewrite List.length_map. lia.
+Qed.
+
+(* Idea: If zero is in the list, then let the left most ν bubble upwards
+         towards the corresponding link until AxCut applies *)
+Lemma link_list_with_0_reduces' :
+  forall n k,
+    k <= n ->
+      forall xs Γ P,
+        length xs = k -> Γ ⊢ P :# ->
+          List.In 0 xs -> link_list xs P -> exists P', P ⊳ P'.
+Proof.
+  induction n; intros.
+  + assert (k = 0) by lia; subst. rewrite List.length_zero_iff_nil in H4; subst. inversion H2.
+  + destruct xs. inversion H3.
+    destruct xs.
+    - inversion H3; simpl in H7; inversion H7.
+    - destruct (PeanoNat.Nat.eq_dec 0 n0).
+      { eapply link_list_with_0_at_0_reduces; rewrite <- e in H3; eauto. }
+      {
+        destruct (PeanoNat.Nat.eq_dec 0 n1).
+        + (* n0 <> 0 /\ n1 = 0 *)
+          eapply link_list_with_0_at_1_reduces; eauto. rewrite <- e in H3; eauto.
+        + (* n0 <> 0 /\ n1 <> 0 *)
+          assert (List.In 0 xs). { simpl in H2; destruct H2 as [|[|]]; congruence. }
+          destruct (link_list_swap_0_1 _ _ _ _ _ n2 n3 H1 H4 H3) as [Q' [Q'' [xs' [? [? [? ?]]]]]].
+          assert (length xs' <= n). { simpl in *; lia. }
+          assert (exists Γ', Γ' ⊢ Q'' :#).
+          { apply ((proj1 struct_cong_preserves_typing) _ _ H5 _) in H1. inversion H1; eexists; eauto. }
+          destruct H10 as [Γ' ?].
+          destruct (IHn _ H9 xs' _ _ eq_refl H10 H7 H6) as [Q''' ?].
+          eexists. eapply r_struct.
+          - apply H5.
+          - eapply r_struct.
+            * eapply c_cut_comm.
+            * eapply r_cong_cut; eauto.
+            * eapply c_cut_comm.
+          - apply c_refl.
+      }
+Qed.
+
+Lemma link_list_with_0_reduces :
+  forall xs Γ P,
+    Γ ⊢ P :# -> List.In 0 xs -> link_list xs P -> exists P', P ⊳ P'.
+Proof.
+  intros.
+  eapply (link_list_with_0_reduces' (length xs) (length xs)); eauto.
+Qed.
+
+Lemma decide_cut_list_link_list :
+  forall Γ P, Γ ⊢ P :# -> cut_list P ->
+    (exists xs, link_list xs P) \/ (exists P', P ⊳ P').
+Proof.
+  intros.
+  generalize dependent Γ.
+  induction H0; intros.
+  + destruct L; destruct R;
+    try match goal with
+    | [ H : no_root_cut (cut ?X ?Y) |- _ ] => unfold no_root_cut in H; specialize H with X Y; congruence
+    end;
+    inversion H1; subst;
+    try ( match goal with [ H : (?A .: ?Γ) ⊢ stop :# |- _ ] => inversion H; ctx_eq_contra end ).
+    - apply link_reduces_or_contains_future in H6.
+      apply link_reduces_or_contains_future in H7.
+      destruct H6 as [[P' ?] | [i1 ?]].
+      * right. exists (cut P' (link m1 m2)). apply r_cong_cut; auto.
+      * destruct H7 as [[P'' ?] | [i2 ?]].
+        ** right. exists (cut (link m m0) P''). eapply r_struct.
+           -- apply c_cut_comm.
+           -- apply r_cong_cut; eauto.
+           -- apply c_cut_comm.
+        ** left. destruct H2; destruct H3; subst; exists [i1; i2]; econstructor.
+    - right.
+      exists (cut (link m m0) (subst_process R ((prefix s) ⋅ id_subst))).
+      eapply r_struct.
+      * eapply c_cut_comm.
+      * eapply r_cong_cut; econstructor.
+      * apply c_cut_comm.
+    - right.
+      exists (cut (subst_process L ((prefix s) ⋅ id_subst)) (link m m0)).
+      apply r_cong_cut; econstructor.
+    - right.
+      exists (cut (subst_process L ((prefix s) ⋅ id_subst)) (seq R s0)).
+      apply r_cong_cut; econstructor.
+  + inversion H1; subst.
+    destruct (IHcut_list _ H7).
+    - destruct L.
+      * (* Lemma : well-typed link either reduces or has a future *)
+        apply link_reduces_or_contains_future in H6.
+        destruct H6 as [[P' ?] | [i ?]].
+        ** right. exists (cut P' P). apply r_cong_cut; auto.
+        ** destruct H2 as [xs' ?].
+           destruct (List.in_dec PeanoNat.Nat.eq_dec 0 xs').
+           {  (* 0 in xs', i.e. we can reduce P *)
+              destruct (link_list_with_0_reduces _ _ _ H7 i0 H2) as [P' ?].
+              right. exists (cut (link m m0) P'). eapply r_struct.
+              + eapply c_cut_comm.
+              + eapply r_cong_cut; eauto.
+              + apply c_cut_comm.
+           }
+           { (* 0 ∉ xs', we use xs'' = pred xs' *)
+             left. exists (i :: (List.map pred xs')).
+             destruct H3; subst.
+             + apply link_cons_l.
+               rewrite List.map_map.
+               assert ( forall a, List.In a xs' -> (fun x : nat => S (Init.Nat.pred x)) a = id a ).
+               { intros. destruct a; auto. congruence. }
+               rewrite ((proj2 List.map_ext_in_iff) H3).
+               rewrite List.map_id; auto.
+             + apply link_cons_r.
+               rewrite List.map_map.
+               assert ( forall a, List.In a xs' -> (fun x : nat => S (Init.Nat.pred x)) a = id a ).
+               { intros. destruct a; auto. congruence. }
+               rewrite ((proj2 List.map_ext_in_iff) H3).
+               rewrite List.map_id; auto.
+           }
+      * exfalso. unfold no_root_cut in H; try congruence.
+      * right. exists (cut (subst_process L ((prefix s) ⋅ id_subst)) P).
+        apply r_cong_cut; econstructor.
+      * inversion H6; ctx_eq_contra.
+    - destruct H2 as [P' ?].
+      right. exists (cut L P').
+      eapply r_struct.
+      * eapply c_cut_comm.
+      * eapply r_cong_cut; eauto.
+      * apply c_cut_comm.
+Qed.
+
+Corollary cut_list_final_or_reduces :
+  forall Γ P, Γ ⊢ P :# -> cut_list P -> final P \/ (exists P', P ⊳ P').
+Proof.
+  intros Γ P Hwt Hct.
+  destruct (decide_cut_list_link_list _ _ Hwt Hct).
+  + destruct H as [xs H0].
+    destruct xs. inversion H0. destruct xs.
+    - left. inversion H0; subst; inversion H3.
+    - destruct (List.in_dec PeanoNat.Nat.eq_dec 0 (n :: n0 :: xs)).
+      * right. apply (link_list_with_0_reduces (n :: n0 :: xs) _ _ Hwt); auto.
+      * left. eapply final_list; eauto. apply c_refl.
+  + right; auto.
+Qed.
+
+(******************************************************************************)
+(* Properties about Irreducible Processes                                     *)
+(******************************************************************************)
+(* 
+Inductive struct_cong_d : nat -> process -> process -> Prop :=
+  (* axioms for equivalence of processes *)
+  | c_link_d : forall ml mr,
+              struct_cong_d 0 (link ml mr) (link mr ml)
+  | c_cut_comm_d : forall P Q,
+                  struct_cong_d 0 (cut P Q) (cut Q P)
+  | c_cut_assoc_d : forall P Q R P' Q' R',
+                    ~ (1 ∈ P) /\ ~ (1 ∈ R') -> (* these premises guarantee that the typing judgements have the proper form *)
+                    P' = down (rename_process P swap01) ->
+                    Q' = rename_process Q swap01 ->
+                    R' = rename_process (up R) swap01 ->
+                    struct_cong_d 0 (cut (cut P Q) R) (cut P' (cut Q' R'))
+
+  (* rules to make the relation an equivalence *)
+  | c_refl_d : forall P, struct_cong_d 0 P P
+  | c_comm_d : forall n P Q, struct_cong_d n P Q -> struct_cong_d (S n) Q P
+  | c_trans_d : forall n1 n2 P Q R,
+                struct_cong_d n1 P Q ->
+                struct_cong_d n2 Q R ->
+                struct_cong_d (S (Nat.max n1 n2)) P R
+
+  (* rules to make the relation a congruence *)
+  | c_cong_link_d : forall n1 m1 m1' n2 m2 m2',
+                    struct_congM_d n1 m1 m1' ->
+                    struct_congM_d n2 m2 m2' ->
+                    struct_cong_d (S (Nat.max n1 n2)) (link m1 m2) (link m1' m2')
+  | c_cong_cut_d : forall n1 P P' n2 Q Q',
+                  struct_cong_d n1 P P' ->
+                  struct_cong_d n2 Q Q' ->
+                  struct_cong_d (S (Nat.max n1 n2)) (cut P Q) (cut P' Q')
+  | c_cong_seq_d : forall n1 P P' n2 s s',
+                  struct_cong_d n1 P P' ->
+                  struct_congS_d n2 s s' ->
+                  struct_cong_d (S (Nat.max n1 n2)) (seq P s) (seq P' s')
+
+with struct_congM_d : nat -> message -> message -> Prop :=
+  | c_cong_fut_d : forall n, struct_congM_d 0 (future n) (future n)
+  | c_cong_prefix_d : forall n s s', struct_congS_d n s s' -> struct_congM_d (S n) (prefix s) (prefix s')
+
+with struct_congS_d : nat -> statement -> statement -> Prop :=
+  | c_cong_choose_l_d : forall n P P',
+                        struct_cong_d n P P' ->
+                        struct_congS_d (S n) (choose_left P) (choose_left P')
+  | c_cong_choose_r_d : forall n P P',
+                        struct_cong_d n P P' ->
+                        struct_congS_d (S n) (choose_right P) (choose_right P')
+  | c_cong_choice_d : forall n1 P P' n2 Q Q',
+                      struct_cong_d n1 P P' ->
+                      struct_cong_d n2 Q Q' ->
+                      struct_congS_d (S (Nat.max n1 n2)) (offer_choice P Q) (offer_choice P' Q')
+  | c_cong_send_d : forall n1 P P' n2 Q Q',
+                    struct_cong_d n1 P P' ->
+                    struct_cong_d n2 Q Q' ->
+                    struct_congS_d (S (Nat.max n1 n2)) (send P Q) (send P' Q')
+  | c_cong_receive_d : forall n P P', struct_cong_d n P P' -> struct_congS_d (S n) (receive P) (receive P')
+  | c_cong_close_d : struct_congS_d 0 close close
+  | c_cong_wait_d : forall n P P', struct_cong_d n P P' -> struct_congS_d (S n) (wait P) (wait P').
+
+Scheme struct_congP_depth_ind := Induction for struct_cong_d Sort Prop
+  with struct_congM_depth_ind := Induction for struct_congM_d Sort Prop
+  with struct_congS_depth_ind := Induction for struct_congS_d Sort Prop.
+Combined Scheme struct_cong_depth_ind from struct_congP_depth_ind, struct_congM_depth_ind, struct_congS_depth_ind.
+
+Lemma struct_cong_d_from_struct_cong :
+  (forall P P', P ≡ P' -> exists k, struct_cong_d k P P') /\
+  (forall M M', M !≡ M' -> exists k, struct_congM_d k M M') /\
+  (forall s s', s $≡ s' -> exists k, struct_congS_d k s s').
+Proof.
+  apply struct_cong_ind; intros;
+    try (now (exists 0; econstructor; eauto));
+    try (now (destruct H; exists (S x); econstructor; eauto)).
+  + destruct H; destruct H0. exists (S (Nat.max x x0)).
+    eapply c_trans_d; eauto.
+  + destruct H; destruct H0. exists (S (Nat.max x x0)).
+    eapply c_cong_link_d; eauto.
+  + destruct H; destruct H0. exists (S (Nat.max x x0)).
+    eapply c_cong_cut_d; eauto.
+  + destruct H; destruct H0. exists (S (Nat.max x x0)).
+    eapply c_cong_seq_d; eauto.
+  + destruct H; destruct H0. exists (S (Nat.max x x0)).
+    eapply c_cong_choice_d; eauto.
+  + destruct H; destruct H0. exists (S (Nat.max x x0)).
+    eapply c_cong_send_d; eauto.
+Qed.
+
+Definition irreducible P := forall Q, ~ (P ⊳ Q).
+
+Lemma stop_equiv_stop_d :
+  forall P n, (forall k, k <= n -> struct_cong_d k stop P \/ struct_cong_d k P stop -> P = stop).
+Proof.
+  intros.
+  generalize dependent k.
+  generalize dependent P.
+  induction n; intros.
+  + inversion H; subst. destruct H0; inversion H0; auto.
+  + destruct H0.
+    - inversion H0; subst; auto.
+      * assert (n0 <= n) by lia.
+        apply (IHn _ _ H2).
+        right; auto.
+      * assert (Q = stop).
+        {
+          assert (n1 <= n) by lia.
+          apply (IHn _ _ H3).
+          left; auto.
+        }
+        subst.
+        assert (n2 <= n) by lia.
+        apply (IHn _ _ H3).
+        left; auto.
+    - inversion H0; subst; auto.
+      * assert (n0 <= n) by lia.
+        apply (IHn _ _ H2).
+        left; auto.
+      * assert (Q = stop).
+        {
+          assert (n2 <= n) by lia.
+          apply (IHn _ _ H3).
+          right; auto.
+        }
+        subst.
+        assert (n1 <= n) by lia.
+        apply (IHn _ _ H3).
+        right; auto.
+Qed.
+
+Lemma stop_equiv_stop : forall P, stop ≡ P -> P = stop.
+Proof.
+  intros. apply struct_cong_d_from_struct_cong in H.
+  destruct H.
+  apply (stop_equiv_stop_d P x x (Nat.le_refl x)); left; auto.
+Qed.
+
+Lemma stop_irreducible : forall P, P = stop -> irreducible P.
+Proof.
+  intros P Hstop Q Hred.
+  induction Hred; try discriminate; subst.
+  apply IHHred.
+  apply stop_equiv_stop; auto.
+Qed.
+
+Lemma link_future_equiv_link_future :
+  forall i M P n,
+    struct_cong_d n (link (future i) M) P \/ struct_cong_d n P (link (future i) M) ->
+    exists M' n', struct_congM_d n' M' M /\ (P = (link (future i) M') \/ P = (link M' (future i))).
+Proof.
+  intros.
+  generalize dependent P.
+  generalize dependent M.
+  induction n; intros.
+  + destruct H.
+    - inversion H; subst.
+      * exists M. admit.
+      * exists M. admit.
+    - inversion H; subst.
+      * admit.
+      * admit.
+  + destruct H.
+    - inversion H; subst.
+Admitted.
+
+
+Lemma link_future_irreducible :
+  forall i M P,
+    P ≡ (link (future i) M) ->
+    irreducible P.
+Proof.
+Admitted.
+
+Lemma ax_cut_inversion_not_0 :
+  forall M P Q i,
+    i <> 0 ->
+    cut (link (future i) M) P ⊳ Q ->
+    exists P', P ⊳ P'.
+Proof.
+Admitted.
+
+
+Lemma link_chain_irreducible :
+  forall P xs,
+    (forall x, List.In x xs -> x <> 0) ->
+    link_chain xs P ->
+    irreducible P.
+Proof.
+  intros.
+  intros Q Hred.
+  induction H0.
+  + apply (stop_irreducible stop eq_refl Q); auto.
+  + assert (i <> 0). { specialize H with i; simpl in H; apply H; auto. }
+    inversion Hred; subst.
+    admit.
+  + admit.
+Admitted. *)
+
+(* argue as follows:
+   use link_tree (similar to link_list but all future of links are free by construction)
+   show that link_treenes is preserved under struct cong
+   then by induction on depth of red relation, show that every link_tree is irred
+   every link_list is a special case of a link_tree, thus irreducbile
+*)
+(* Lemma final_iff_irreducible :
+  forall Γ P, Γ ⊢ P :# -> (final P <-> irreducible P).
+Proof.
+  intros; split.
+  + intro Hfinal. destruct Hfinal as [xs P P' Hnzero Hchain Hequiv].
+    induction Hchain.
+    - apply stop_irreducible.
+      apply c_comm in Hequiv.
+      apply stop_equiv_stop; auto.
+    - admit.
+    - admit.
+  + intro Hirred. *)
