formalization/Progress.v
@@ -1,0 +1,70 @@
+From FD Require Import Syntax.
+From FD Require Import Types.
+From FD Require Import StructCong.
+From FD Require Import Reduction.
+From FD Require Import Contexts.
+From FD Require Import Typing.
+From FD Require Import FreeVars.
+From FD Require Import FinalProcess.
+
+From Stdlib Require Import Lia.
+
+Theorem progress :
+  forall Γ P, Γ ⊢ P :# -> (exists P', P ⊳ P') \/ final P.
+Proof.
+  intros.
+  induction H.
+  + apply or_comm.
+    apply (link_final_or_reduces _ _ _ (t_ax _ _ _ _ _ _ H H0 H1)).
+  + (* restructure cut into canonical form *)
+    assert (Γ ⊢ (cut P Q) :# ) by (econstructor; eauto).
+    destruct (canonical_cut_form _ _ _ H2) as [P' [? ?]].
+
+    (* decide whether canonical form is final or reduces *)
+    assert (Γ ⊢ P' :#). { apply ((proj1 struct_cong_preserves_typing) _ _ H3) in H2; auto. }
+    destruct (cut_list_final_or_reduces _ _ H5 H4).
+    - inversion H6; subst.
+      * inversion H4.
+      * inversion H4.
+      * inversion H4.
+      * right. eapply final_list; eauto.
+        eapply c_trans; eauto.
+    - destruct H6 as [P'' ?].
+      left. exists P''. eapply r_struct; eauto. apply c_refl.
+  + left.
+    exists (subst_process P ((prefix s) ⋅ id_subst)).
+    econstructor.
+  + right. econstructor.
+Qed.
+
+Corollary progress_for_closed_processes :
+  forall Γ P, ctx_eq Γ empty_ctx -> Γ ⊢ P :# -> (exists P', P ⊳ P') \/ (P = stop).
+Proof.
+  intros.
+  destruct (progress _ _ H0); auto.
+  right. inversion H1; subst; auto;
+  exfalso.
+  + assert (i ∈ link (future i) M) by repeat econstructor.
+    assert (~ i ∈ link (future i) M).
+    { apply ((proj1 ctx_none_not_free) _ _ _ H0). apply ctx_lookup_eq_empty; auto. }
+    congruence.
+  + assert (i ∈ link M (future i)). { apply fv_link_r; econstructor. }
+    assert (~ i ∈ link M (future i)).
+    { apply ((proj1 ctx_none_not_free) _ _ _ H0). apply ctx_lookup_eq_empty; auto. }
+    congruence.
+  + destruct xs.
+    - inversion H3.
+    - apply (proj1 struct_cong_preserves_typing _ _ H4) in H0.
+      assert ((Nat.pred n) ∈ P').
+      {
+        apply (link_list_free_vars _ (n :: xs)); auto.
+        + intros. destruct x; try lia. congruence.
+        + left; auto.
+      }
+      assert (~ (Nat.pred n) ∈ P').
+      {
+        apply ((proj1 ctx_none_not_free) _ _ _ H0).
+        apply ctx_lookup_eq_empty; auto.
+      }
+      congruence.
+Qed.
